Step-index in bigstep relation is now a different letter to avoid confusion

src/Language/PlutusIR/Semantics/Dynamic/Bigstep.v
@@ -10,104 +10,104 @@ Require Export PlutusCert.Language.PlutusIR.Semantics.Dynamic.Values.
 (** * Big-step operational semantics *)
 
 (** ** Implementation of big-step semantics as an inductive datatype *)
-Reserved Notation "t '=[' k ']=>' v"(at level 40).
+Reserved Notation "t '=[' j ']=>' v"(at level 40).
 Inductive eval : Term -> Term -> nat -> Prop :=
   (** Let-bindings *)
-  | E_Let : forall bs t v k,
-      eval_bindings_nonrec (Let NonRec bs t) v k->
-      (Let NonRec bs t) =[k]=> v
-  | E_LetRec : forall bs t v k,
-      eval_bindings_rec bs (Let Rec bs t) v k->
-      (Let Rec bs t) =[k]=> v
+  | E_Let : forall bs t v j,
+      eval_bindings_nonrec (Let NonRec bs t) v j ->
+      (Let NonRec bs t) =[j]=> v
+  | E_LetRec : forall bs t v j ,
+      eval_bindings_rec bs (Let Rec bs t) v j ->
+      (Let Rec bs t) =[j]=> v
   (** Others *)
   | E_TyAbs : forall X K t,
       TyAbs X K t =[0]=> TyAbs X K t
   | E_LamAbs : forall x T t,
       LamAbs x T t =[0]=> LamAbs x T t
-  | E_Apply : forall t1 t2 x T t0 v2 v0 k1 k2 k0,
-      t1 =[k1]=> LamAbs x T t0 ->
-      t2 =[k2]=> v2 ->
-      <{ [v2 / x] t0 }> =[k0]=> v0 ->
-      Apply t1 t2 =[k1 + k2 + 1 + k0]=> v0
+  | E_Apply : forall t1 t2 x T t0 v2 v0 j1 j2 j0,
+      t1 =[j1]=> LamAbs x T t0 ->
+      t2 =[j2]=> v2 ->
+      <{ [v2 / x] t0 }> =[j0]=> v0 ->
+      Apply t1 t2 =[j1 + j2 + 1 + j0]=> v0
   | E_Constant : forall a,
       Constant a =[0]=> Constant a
   (* Builtins *)
   | E_Builtin : forall f,
       Builtin f =[0]=> Builtin f
-  | E_ApplyBuiltin1 : forall t1 t2 v1 v2 k1 k2,
-      t1 =[k1]=> v1 ->
+  | E_ApplyBuiltin1 : forall t1 t2 v1 v2 j1 j2,
+      t1 =[j1]=> v1 ->
       value_builtin v1 ->
-      t2 =[k2]=> v2 ->
+      t2 =[j2]=> v2 ->
       value_builtin (Apply v1 v2) ->
-      Apply t1 t2 =[k1 + k2]=> Apply v1 v2
-  | E_ApplyBuiltin2 : forall t1 t2 v1 v2 v0 k1 k2,
-      t1 =[k1]=> v1 ->
+      Apply t1 t2 =[j1 + j2]=> Apply v1 v2
+  | E_ApplyBuiltin2 : forall t1 t2 v1 v2 v0 j1 j2,
+      t1 =[j1]=> v1 ->
       value_builtin v1 ->
-      t2 =[k2]=> v2 ->
+      t2 =[j2]=> v2 ->
       ~(value_builtin (Apply v1 v2)) ->
       compute_defaultfun (Apply v1 v2) = Datatypes.Some v0 ->
-      Apply t1 t2 =[k1 + k2 + 1]=> v0
+      Apply t1 t2 =[j1 + j2 + 1]=> v0
   (** Builtins: If-Then-Else 
 
       We handle this built-in function separately because it has a unique behaviour:
       The ``then''-branch should only be evaluated when the condition is true,
       and the opposite is true for the ``else''-branch.
   *)
-  | E_IfTyInst : forall t1 T k1,
-      t1 =[k1]=> Builtin IfThenElse ->
-      TyInst t1 T =[k1]=> TyInst (Builtin IfThenElse) T
-  | E_IfCondition : forall t_b t_c T cond k_b k_c,
-      t_b =[k_b]=> TyInst (Builtin IfThenElse) T ->
-      t_c =[k_c]=> Constant (Some (ValueOf DefaultUniBool cond)) ->
-      Apply t_b t_c =[k_b + k_c]=> Apply (TyInst (Builtin IfThenElse) T) (Constant (Some (ValueOf DefaultUniBool cond)))
-  | E_IfThenBranch : forall t_bc t_t T cond k_bc,
-      t_bc =[k_bc]=> Apply (TyInst (Builtin IfThenElse) T) (Constant (Some (ValueOf DefaultUniBool cond))) ->
-      Apply t_bc t_t =[k_bc]=> Apply (Apply (TyInst (Builtin IfThenElse) T) (Constant (Some (ValueOf DefaultUniBool cond)))) t_t
-  | E_IfTrue : forall t_bct t_t T v_t t_e k_bct k_t,
-      t_bct =[k_bct]=> Apply (Apply (TyInst (Builtin IfThenElse) T) (Constant (Some (ValueOf DefaultUniBool true)))) t_t ->
-      t_t =[k_t]=> v_t ->
-      Apply t_bct t_e =[k_bct + k_t]=> v_t
-  | E_IfFalse : forall t_bct t_t T v_e t_e k_bct k_e,
-      t_bct =[k_bct]=> Apply (Apply (TyInst (Builtin IfThenElse) T) (Constant (Some (ValueOf DefaultUniBool false)))) t_t ->
-      t_e =[k_e]=> v_e ->
-      Apply t_bct t_e =[k_bct + k_e]=> v_e
+  | E_IfTyInst : forall t1 T j1,
+      t1 =[j1]=> Builtin IfThenElse ->
+      TyInst t1 T =[j1]=> TyInst (Builtin IfThenElse) T
+  | E_IfCondition : forall t_b t_c T cond j_b j_c,
+      t_b =[j_b]=> TyInst (Builtin IfThenElse) T ->
+      t_c =[j_c]=> Constant (Some (ValueOf DefaultUniBool cond)) ->
+      Apply t_b t_c =[j_b + j_c]=> Apply (TyInst (Builtin IfThenElse) T) (Constant (Some (ValueOf DefaultUniBool cond)))
+  | E_IfThenBranch : forall t_bc t_t T cond j_bc,
+      t_bc =[j_bc]=> Apply (TyInst (Builtin IfThenElse) T) (Constant (Some (ValueOf DefaultUniBool cond))) ->
+      Apply t_bc t_t =[j_bc]=> Apply (Apply (TyInst (Builtin IfThenElse) T) (Constant (Some (ValueOf DefaultUniBool cond)))) t_t
+  | E_IfTrue : forall t_bct t_t T v_t t_e j_bct j_t,
+      t_bct =[j_bct]=> Apply (Apply (TyInst (Builtin IfThenElse) T) (Constant (Some (ValueOf DefaultUniBool true)))) t_t ->
+      t_t =[j_t]=> v_t ->
+      Apply t_bct t_e =[j_bct + j_t]=> v_t
+  | E_IfFalse : forall t_bct t_t T v_e t_e j_bct j_e,
+      t_bct =[j_bct]=> Apply (Apply (TyInst (Builtin IfThenElse) T) (Constant (Some (ValueOf DefaultUniBool false)))) t_t ->
+      t_e =[j_e]=> v_e ->
+      Apply t_bct t_e =[j_bct + j_e]=> v_e
   (* Type instantiation *)
-  | E_TyInst : forall t1 T2 X K t0 v0 k1 k0,
-      t1 =[k1]=> TyAbs X K t0 ->
-      <{ [[T2 / X] t0 }> =[k0]=> v0 ->
-      TyInst t1 T2 =[k1 + 1 + k0]=> v0
+  | E_TyInst : forall t1 T2 X K t0 v0 j1 j0,
+      t1 =[j1]=> TyAbs X K t0 ->
+      <{ [[T2 / X] t0 }> =[j0]=> v0 ->
+      TyInst t1 T2 =[j1 + 1 + j0]=> v0
   (* Errors and their propagation *)
   | E_Error : forall T,
       Error T =[0]=> Error T
   (* Wrap and unwrap *)
-  | E_IWrap : forall F T t0 v0 k0,
-      t0 =[k0]=> v0 ->
-      IWrap F T t0 =[k0]=> IWrap F T v0
-  | E_Unwrap : forall t0 F T v0 k0,
-      t0 =[k0]=> IWrap F T v0 ->
-      Unwrap t0 =[k0 + 1]=> v0
+  | E_IWrap : forall F T t0 v0 j0,
+      t0 =[j0]=> v0 ->
+      IWrap F T t0 =[j0]=> IWrap F T v0
+  | E_Unwrap : forall t0 F T v0 j0,
+      t0 =[j0]=> IWrap F T v0 ->
+      Unwrap t0 =[j0 + 1]=> v0
   (* TODO: Should there be a rule for type reduction? *)
 
   (* TODO: Errors propagate *)
 
 with eval_bindings_nonrec : Term -> Term -> nat -> Prop :=
-  | E_NilB_NonRec : forall t v k,
-      t =[k]=> v ->
-      eval_bindings_nonrec (Let NonRec nil t) v (S k)
-  | E_ConsB_NonRec : forall s x T tb bs t vb v kb k,
-      tb =[kb]=> vb ->
-      eval_bindings_nonrec <{ [vb / x] ({Let NonRec bs t}) }> v k ->
-      eval_bindings_nonrec (Let NonRec ((TermBind s (VarDecl x T) tb) :: bs) t) v (kb + 1 + k)
+  | E_NilB_NonRec : forall t v j,
+      t =[j]=> v ->
+      eval_bindings_nonrec (Let NonRec nil t) v (S j)
+  | E_ConsB_NonRec : forall s x T tb bs t vb v jb j,
+      tb =[jb]=> vb ->
+      eval_bindings_nonrec <{ [vb / x] ({Let NonRec bs t}) }> v j ->
+      eval_bindings_nonrec (Let NonRec ((TermBind s (VarDecl x T) tb) :: bs) t) v (jb + 1 + j)
 
 with eval_bindings_rec : list Binding -> Term -> Term -> nat -> Prop :=
-  | E_NilB_Rec : forall bs0 t v k,
-      t =[k]=> v ->
-      eval_bindings_rec bs0 (Let Rec nil t) v (S k)
-  | E_ConsB_Rec : forall bs0 s x T tb bs t v k,
-      eval_bindings_rec bs0 <{ [ {Let Rec bs0 tb} / x] {Let Rec bs t} }>  v k ->
-      eval_bindings_rec bs0 (Let Rec ((TermBind s (VarDecl x T) tb) :: bs) t) v (k + 1)
+  | E_NilB_Rec : forall bs0 t v j,
+      t =[j]=> v ->
+      eval_bindings_rec bs0 (Let Rec nil t) v (S j)
+  | E_ConsB_Rec : forall bs0 s x T tb bs t v j,
+      eval_bindings_rec bs0 <{ [ {Let Rec bs0 tb} / x] {Let Rec bs t} }>  v j ->
+      eval_bindings_rec bs0 (Let Rec ((TermBind s (VarDecl x T) tb) :: bs) t) v (j + 1)
 
-where "t '=[' k ']=>' v" := (eval t v k).
+where "t '=[' j ']=>' v" := (eval t v j).
 
 Scheme eval__ind := Minimality for eval Sort Prop
   with eval_bindings_nonrec__ind := Minimality for eval_bindings_nonrec Sort Prop
