src/Language/PlutusIR/Semantics/TypeSafety/Preservation.v
@@ -1,5 +1,3 @@
-Require Import PlutusCert.Language.PlutusIR.
-Import NamedTerm.
 Require Import PlutusCert.Language.PlutusIR.Semantics.Static.
 Require Import PlutusCert.Language.PlutusIR.Semantics.Dynamic.
 
